Foundation/Propositional/Hilbert/Corsi/Disjunctive.lean
@@ -116,4 +116,32 @@ instance F_Tra1.KleeneSlashable : Propositional.F_Tra1.KleeneSlashable := Hilber
       . grind;
 instance F_Tra1.Disjunctive : Entailment.Disjunctive Propositional.F_Tra1 := inferInstance
 
+example : ∀ {s : Substitution ℕ}, ∕[(Hilbert.Corsi {Axioms.Per #0})] ((Axioms.Per #0)⟦s⟧) := by
+  intro s;
+  constructor;
+  . sorry;
+  . intro h;
+    constructor;
+    . apply af;
+      generalize #0⟦s⟧ = φ at h ⊢;
+      induction φ with
+      | hatom a => exact h;
+      | hfalsum => contradiction;
+      | hor φ ψ ihφ ihψ => grind;
+      | hand φ ψ ihφ ihpsi => grind;
+      | himp φ ψ ihφ ihψ => exact h.1;
+    . grind;
+
+example : ∀ {s : Substitution ℕ}, ∕[(Hilbert.Corsi {Axioms.Sym #0 #1})] ((Axioms.Sym #0 #1)⟦s⟧) := by
+  intro s;
+  constructor;
+  . sorry;
+  . intro h₁;
+    apply or_iff_not_imp_left.mpr;
+    intro h₂;
+    apply KleeneSlash.def_neg.mpr;
+    constructor;
+    . sorry;
+    . sorry;
+
 end LO.Propositional
